io/TODO.md
@@ -1,0 +1,13 @@
+# Effects
+- [ ] are the effects finished?
+- [ ] can the effects be used to write something useful?
+
+# Extraction
+- [ ] is extracting defined correctly?
+- [ ] arrows can not be ml-ish, therefore we should rethink what is noted
+      with ml
+- [ ] check extraction
+
+# Model & Proof
+- [ ] make sure the model is correct
+- [ ] check the proofs and finish them
